Set up simulation stuff for evaluate_init
Proves most things about expressions except for do_app, and leaves
evaluate_decs results cheated.

compiler/repl/evaluate_initScript.sml
@@ -3,7 +3,11 @@
   holds at initialisation.
 *)
 
-open preamble evaluate_skipTheory
+open preamble
+open evaluateTheory semanticPrimitivesTheory evaluatePropsTheory
+open namespacePropsTheory ml_progTheory
+open evaluate_skipTheory
+local open helperLib in end
 
 val _ = new_theory "evaluate_init";
 
@@ -16,7 +20,1705 @@ Proof
   rw[SUBMAP_FLOOKUP_EQN, FLOOKUP_FUN_FMAP, SUBSET_DEF]
 QED
 
-(* -- *)
+Theorem NOT_NIL_CONS:
+  xs ≠ [] ⇔ ∃y ys. xs = y::ys
+Proof
+  Cases_on ‘xs’ \\ gs []
+QED
+
+(* -------------------------------------------------------------------------
+ *
+ * ------------------------------------------------------------------------- *)
+
+Definition state_ok_def:
+  state_ok (s: 'ffi semanticPrimitives$state) ⇔
+    state_rel (LENGTH s.refs) (FUN_FMAP I (count (LENGTH s.refs)))
+                              (FUN_FMAP I (count s.next_type_stamp))
+                              (FUN_FMAP I (count s.next_exn_stamp)) s s
+End
+
+Definition env_ok_def:
+  env_ok (s: 'ffi semanticPrimitives$state) env ⇔
+    env_rel (FUN_FMAP I (count (LENGTH s.refs)))
+            (FUN_FMAP I (count s.next_type_stamp))
+            (FUN_FMAP I (count s.next_exn_stamp))
+            env env
+End
+
+Definition v_ok_def:
+  v_ok (s: 'ffi semanticPrimitives$state) v ⇔
+    v_rel (FUN_FMAP I (count (LENGTH s.refs)))
+          (FUN_FMAP I (count s.next_type_stamp))
+          (FUN_FMAP I (count s.next_exn_stamp))
+          v v
+End
+
+Definition ref_ok_def:
+  ref_ok (s: 'ffi semanticPrimitives$state) v ⇔
+    ref_rel (v_rel (FUN_FMAP I (count (LENGTH s.refs)))
+                   (FUN_FMAP I (count s.next_type_stamp))
+                   (FUN_FMAP I (count s.next_exn_stamp)))
+                   v v
+End
+
+Theorem ref_ok_thm:
+  ref_ok s (Refv v) = v_ok s v ∧
+  ref_ok s (Varray vs) = EVERY (v_ok s) vs ∧
+  ref_ok s (W8array a) = T
+Proof
+  rw [ref_ok_def, ref_rel_def, v_ok_def, LIST_REL_EL_EQN, EVERY_EL]
+QED
+
+Definition stamp_ok_def:
+  stamp_ok (s: 'ffi semanticPrimitives$state) st ⇔
+    stamp_rel (FUN_FMAP I (count s.next_type_stamp))
+              (FUN_FMAP I (count s.next_exn_stamp)) st st
+End
+
+Theorem evaluate_v_ok_mono:
+  evaluate s env xs = (t, res) ∧
+  v_ok s v ⇒
+    v_ok t v
+Proof
+  rw []
+  \\ drule_then assume_tac (CONJUNCT1 evaluate_next_type_stamp_mono)
+  \\ drule_then assume_tac (CONJUNCT1 evaluate_next_exn_stamp_mono)
+  \\ drule_then assume_tac (CONJUNCT1 evaluate_refs_length_mono)
+  \\ gs [v_ok_def]
+  \\ irule v_rel_update
+  \\ first_assum (irule_at Any)
+  \\ gs [FUN_FMAP_SUBMAP_SUBSET, COUNT_MONO]
+QED
+
+Theorem evaluate_env_ok_mono:
+  evaluate s env xs = (t, res) ∧
+  env_ok s env ⇒
+    env_ok t env
+Proof
+  rw []
+  \\ drule_then assume_tac (CONJUNCT1 evaluate_next_type_stamp_mono)
+  \\ drule_then assume_tac (CONJUNCT1 evaluate_next_exn_stamp_mono)
+  \\ drule_then assume_tac (CONJUNCT1 evaluate_refs_length_mono)
+  \\ gs [env_ok_def]
+  \\ irule env_rel_update
+  \\ first_assum (irule_at Any)
+  \\ gs [FUN_FMAP_SUBMAP_SUBSET, COUNT_MONO]
+QED
+
+Theorem v_ok_thm:
+  (∀opt vs. v_ok s (Conv opt vs) ⇔
+     EVERY (v_ok s) vs ∧
+     (∀st. opt = SOME st ⇒ stamp_ok s st)) ∧
+  (∀env n x. v_ok s (Closure env n x) ⇔ env_ok s env) ∧
+  (∀env f n. v_ok s (Recclosure env f n) ⇔ env_ok s env) ∧
+  (∀vs. v_ok s (Vectorv vs) ⇔ EVERY (v_ok s) vs) ∧
+  (∀lit. v_ok s (Litv lit)) ∧
+  (∀loc. v_ok s (Loc loc) ⇔ loc < LENGTH s.refs) ∧
+  (∀env ns. v_ok s (Env env ns) ⇔ env_ok s env)
+Proof
+  rw [v_ok_def, v_rel_def, OPTREL_def, env_ok_def, FLOOKUP_FUN_FMAP,
+      LIST_REL_EL_EQN, EVERY_EL, stamp_ok_def]
+  \\ rw [EQ_IMP_THM] \\ gs []
+  \\ Cases_on ‘opt’ \\ gs []
+QED
+
+local
+  val ind_thm =
+    full_evaluate_ind
+    |> Q.SPECL [
+      ‘λs env xs. ∀t res.
+        evaluate s env xs = (t, res) ∧
+        state_ok s ∧
+        env_ok s env ∧
+        res ≠ Rerr (Rabort Rtype_error) ⇒
+          state_ok t ∧
+          env_ok t env ∧
+          (∀vs. res = Rval vs ⇒ EVERY (v_ok t) vs) ∧
+          (∀v. res = Rerr (Rraise v) ⇒ v_ok t v)’,
+      ‘λs env v ps errv. ∀t res.
+        evaluate_match s env v ps errv = (t, res) ∧
+        state_ok s ∧
+        env_ok s env ∧
+        v_ok s v ∧
+        v_ok s errv ∧
+        res ≠ Rerr (Rabort Rtype_error) ⇒
+          state_ok t ∧
+          env_ok t env ∧
+          (∀vs. res = Rval vs ⇒ EVERY (v_ok t) vs) ∧
+          (∀v. res = Rerr (Rraise v) ⇒ v_ok t v)’,
+      ‘λs env ds. ∀t res.
+        evaluate_decs s env ds = (t, res) ∧
+        state_ok s ∧
+        env_ok s env ∧
+        res ≠ Rerr (Rabort Rtype_error) ⇒
+          state_ok t ∧
+          env_ok t env ∧
+          (∀env. res = Rval env ⇒ env_ok t env) ∧
+          (∀v. res = Rerr (Rraise v) ⇒ v_ok t v)’ ]
+    |> CONV_RULE (DEPTH_CONV BETA_CONV);
+  val ind_goals =
+    ind_thm |> concl |> dest_imp |> fst
+            |> helperLib.list_dest dest_conj
+in
+  fun get_goal s =
+    first (can (find_term (can (match_term (Term [QUOTE s]))))) ind_goals
+    |> helperLib.list_dest dest_forall
+    |> last
+  fun evaluate_ok () = ind_thm |> concl |> rand
+  fun the_ind_thm () = ind_thm
+end
+
+Theorem evaluate_ok_Nil:
+  ^(get_goal "[]")
+Proof
+  rw [evaluate_def] \\ gs []
+QED
+
+Theorem evaluate_ok_Cons:
+  ^(get_goal "_::_::_")
+Proof
+  rw [evaluate_def]
+  \\ gvs [CaseEqs ["result", "prod"]]
+  \\ drule_then strip_assume_tac evaluate_sing \\ gvs []
+  \\ irule evaluate_v_ok_mono \\ gs [SF SFY_ss]
+QED
+
+Theorem evaluate_ok_Lit:
+  ^(get_goal "Lit l")
+Proof
+  rw [evaluate_def] \\ gs []
+  \\ simp [v_ok_thm]
+QED
+
+Theorem evaluate_ok_Raise:
+  ^(get_goal "Raise e")
+Proof
+  rw [evaluate_def] \\ gs []
+  \\ gvs [CaseEqs ["result", "prod"]]
+  \\ drule_then strip_assume_tac evaluate_sing \\ gvs []
+QED
+
+Theorem evaluate_ok_Handle:
+  ^(get_goal "Handle e")
+Proof
+  rw [evaluate_def]
+  \\ gvs [CaseEqs ["prod", "result", "error_result", "bool"]]
+QED
+
+Theorem evaluate_ok_Con:
+  ^(get_goal "Con cn es")
+Proof
+  rw [evaluate_def]
+  \\ gvs [CaseEqs ["prod", "result", "option"]]
+  \\ gvs [build_conv_def, CaseEqs ["option", "prod"], v_ok_thm]
+  \\ gs [env_ok_def, env_rel_def, stamp_ok_def, ctor_rel_def]
+  \\ drule_all_then strip_assume_tac nsAll2_nsLookup1 \\ gs []
+  \\ irule stamp_rel_update
+  \\ first_assum (irule_at Any)
+  \\ drule_then assume_tac (CONJUNCT1 evaluate_next_type_stamp_mono)
+  \\ drule_then assume_tac (CONJUNCT1 evaluate_next_exn_stamp_mono)
+  \\ gs [FUN_FMAP_SUBMAP_SUBSET, COUNT_MONO]
+QED
+
+Theorem evaluate_ok_Var:
+  ^(get_goal "ast$Var n")
+Proof
+  rw [evaluate_def]
+  \\ gvs [CaseEqs ["option"]]
+  \\ gs [env_ok_def, env_rel_def, v_ok_def]
+  \\ drule_all_then strip_assume_tac nsAll2_nsLookup1 \\ gs []
+QED
+
+Theorem evaluate_ok_Fun:
+  ^(get_goal "ast$Fun n e")
+Proof
+  rw [evaluate_def]
+  \\ gvs [CaseEqs ["option"], v_ok_thm]
+QED
+
+Theorem state_ok_eval_state:
+  state_ok s ⇒ s.eval_state = NONE
+Proof
+  rw [state_ok_def, state_rel_def]
+QED
+
+Theorem do_eval_state_none:
+  s.eval_state = NONE ⇒
+    do_eval_res vs s =
+      (s, (Rerr (Rabort Rtype_error) : (v sem_env # dec list, v) result))
+Proof
+  rw [do_eval_res_def, do_eval_def]
+QED
+
+Theorem evaluate_ok_Eval:
+  op = Eval ⇒ ^(get_goal "App")
+Proof
+  simp [evaluate_def]
+  \\ strip_tac
+  \\ strip_tac
+  \\ rpt gen_tac
+  \\ strip_tac
+  \\ qpat_x_assum ‘_ = (t,res)’ mp_tac
+  \\ TOP_CASE_TAC \\ rfs []
+  \\ reverse TOP_CASE_TAC \\ rfs []
+  >- (
+    rw [] \\ gs [])
+  \\ drule_then assume_tac state_ok_eval_state
+  \\ drule_then assume_tac do_eval_state_none
+  \\ simp []
+QED
+
+Theorem v_ok_v_to_list:
+  ∀v vs.
+    v_ok s v ∧
+    state_ok s ∧
+    v_to_list v = SOME vs ⇒
+      EVERY (v_ok s) vs
+Proof
+  ho_match_mp_tac v_to_list_ind \\ gs []
+  \\ rw [] \\ gvs [v_ok_thm]
+  \\ gvs [v_to_list_def, CaseEq "option"]
+QED
+
+Theorem v_rel_list_to_v:
+  ∀v vs.
+    v_to_list v = SOME vs ∧
+    state_ok s ∧
+    v_ok s v ⇒
+      EVERY (v_ok s) vs
+Proof
+  ho_match_mp_tac v_to_list_ind
+  \\ rw [] \\ gvs [v_ok_thm, v_to_list_def, CaseEq "option"]
+QED
+
+Theorem do_app_cases[local] = semanticPrimitivesPropsTheory.do_app_cases;
+
+Theorem state_ok_refs_ok:
+  state_ok s ⇒ EVERY (ref_ok s) s.refs
+Proof
+  rw [state_ok_def, ref_ok_def, state_rel_def, EVERY_EL]
+  \\ first_x_assum (qspec_then ‘n’ assume_tac) \\ gs []
+QED
+
+Theorem do_app_update:
+  do_app (s.refs,s.ffi) op vs = SOME ((refs,ffi), res) ∧
+  state_ok s ∧
+  EVERY (v_ok s) vs ∧
+  op ≠ Opapp ∧
+  op ≠ Eval ⇒
+    let t = (s with <| refs := refs; ffi := ffi |>) in
+    state_ok t ∧
+    EVERY (ref_ok t) refs ∧
+    (∀v. res = Rval v ⇒ v_ok t v) ∧
+    (∀v. res = Rerr (Rraise v) ⇒ v_ok t v)
+Proof
+  cheat (*
+  strip_tac
+  \\ drule_then assume_tac state_ok_refs_ok
+  \\ Cases_on ‘op = Env_id’ \\ gs []
+  >- (
+    gvs [do_app_cases, v_ok_thm]
+    \\ first_x_assum (irule_at Any) \\ gs [v_ok_thm, nat_to_v_def])
+  \\ Cases_on ‘∃chn. op = FFI chn’ \\ gs []
+  >- (
+    gvs [do_app_cases, v_ok_thm, ffiTheory.call_FFI_def, store_assign_def,
+         store_lookup_def,
+         CaseEqs ["ffi_result", "option", "bool", "oracle_result"]]
+    \\ cheat)
+    >- (
+      qmatch_goalsub_abbrev_tac ‘_ :'a ffi_state = ffi2’
+      \\ Q.REFINE_EXISTS_TAC ‘s with <| refs := r; ffi := f |>’ \\ simp []
+      \\ simp [EVERY_LUPDATE]
+    \\ simp
+    \\ first_x_assum (irule_at Any)
+    \\ gs [st]
+    \\ first_x_assum (irule_at Any) \\ gs [v_ok_thm, nat_to_v_def])
+    Cases_on ‘res’ \\ gvs [do_app_def, v_rel_def, OPTREL_def,
+                           CaseEqs ["list", "v", "option", "prod", "lit",
+                                    "store_v"], PULL_EXISTS]
+    \\ rpt (irule_at Any SUBMAP_REFL) \\ gs []
+    \\ drule_all_then assume_tac state_rel_store_lookup
+    \\ ‘t.ffi = s.ffi’
+      by gs [state_rel_def]
+    \\ gs [OPTREL_def]
+    \\ rename1 ‘ref_rel _ _ y0’ \\ Cases_on ‘y0’ \\ gvs [ref_rel_def]
+    >- (
+      gvs [CaseEqs ["ffi_result", "option", "bool", "oracle_result"],
+              ffiTheory.call_FFI_def, PULL_EXISTS, state_rel_def]
+      \\ gs [store_assign_def, store_lookup_def, v_rel_def])
+    \\ gvs [CaseEqs ["ffi_result", "option", "bool", "oracle_result"],
+            ffiTheory.call_FFI_def, PULL_EXISTS, EXISTS_PROD, v_rel_def,
+            store_assign_def, store_lookup_def]
+    \\ Q.REFINE_EXISTS_TAC
+      ‘<| refs := r1; ffi := f1; clock := s.clock;
+          next_type_stamp := nts1; next_exn_stamp := nes1;
+          eval_state := NONE |>’ \\ gs []
+    \\ Q.REFINE_EXISTS_TAC
+      ‘<| refs := r2; ffi := f2; clock := t.clock;
+          next_type_stamp := nts2; next_exn_stamp := nes2;
+          eval_state := NONE |>’ \\ gs []
+    \\ gs [state_rel_def, EL_LUPDATE]
+    \\ qx_gen_tac ‘n1’ \\ rw [] \\ gs [ref_rel_def]
+    \\ first_x_assum (qspec_then ‘n1’ assume_tac) \\ gs []
+    \\ rw [] \\ gs []
+    \\ qpat_x_assum ‘INJ ($' fr) _ _’ mp_tac \\ rw [INJ_DEF]
+    \\ qpat_x_assum ‘FLOOKUP fr _ = _’ mp_tac \\ rw [flookup_thm]
+    \\ qpat_x_assum ‘FLOOKUP fr _ = _’ mp_tac \\ rw [flookup_thm]
+    \\ gs [])
+  \\ Cases_on ‘op = ConfigGC’ \\ gs []
+  >- (
+    Cases_on ‘res’ \\ gvs [do_app_def, v_rel_def, OPTREL_def,
+                           CaseEqs ["list", "v", "option", "prod", "lit"]]
+    \\ rpt (irule_at Any SUBMAP_REFL) \\ gs []
+    \\ first_assum (irule_at Any) \\ gs [])
+  \\ Cases_on ‘op = ListAppend’ \\ gs []
+  >- (
+    ‘FLOOKUP ft list_type_num = SOME list_type_num ∧
+     INJ ($' ft) (FDOM ft) (count t.next_type_stamp) ∧
+     list_type_num < t.next_type_stamp’
+      by (gs [state_rel_def]
+          \\ qpat_x_assum ‘INJ ($' ft) _ _’ mp_tac \\ rw [INJ_DEF]
+          \\ rpt (first_x_assum (qspec_then ‘list_type_num’ assume_tac))
+          \\ gs [flookup_thm])
+    \\ Cases_on ‘res’ \\ gvs [do_app_def, v_rel_def, OPTREL_def,
+                              CaseEqs ["list", "v", "option", "prod", "lit"]]
+    \\ rpt (irule_at Any SUBMAP_REFL) \\ gs []
+    \\ dxrule v_rel_v_to_list
+    \\ rpt (disch_then drule) \\ gs []
+    \\ disch_then drule \\ rw [OPTREL_def]
+    \\ gs [option_nchotomy]
+    \\ dxrule v_rel_v_to_list
+    \\ rpt (disch_then drule) \\ gs []
+    \\ disch_then drule \\ rw [OPTREL_def]
+    \\ first_assum (irule_at Any)
+    \\ first_assum (irule_at Any) \\ gs []
+    \\ irule v_rel_list_to_v \\ gs []
+    \\ irule_at Any v_to_list_list_to_v
+    \\ irule_at Any v_to_list_list_to_v
+    \\ gs [LIST_REL_EL_EQN, EL_APPEND_EQN]
+    \\ rw [] \\ gs[])
+  \\ Cases_on ‘op = Aw8sub_unsafe’ \\ gs []
+  >- (
+    Cases_on ‘res’ \\ gvs [do_app_def, v_rel_def, OPTREL_def,
+                           CaseEqs ["list", "v", "option", "prod", "lit",
+                                    "store_v"]]
+    \\ rpt (irule_at Any SUBMAP_REFL) \\ gs []
+    \\ drule_all_then assume_tac state_rel_store_lookup \\ gs [OPTREL_def]
+    \\ rename1 ‘ref_rel _ _ y0’ \\ Cases_on ‘y0’ \\ gs [ref_rel_def]
+    \\ rw [] \\ gs []
+    \\ first_assum (irule_at Any) \\ gs [v_rel_def])
+  \\ Cases_on ‘op = Aw8update_unsafe’ \\ gs []
+  >- (
+    Cases_on ‘res’ \\ gvs [do_app_def, v_rel_def, OPTREL_def,
+                           CaseEqs ["list", "v", "option", "prod", "lit",
+                                    "store_v"]]
+    \\ rpt (irule_at Any SUBMAP_REFL) \\ gs []
+    \\ drule_all_then assume_tac state_rel_store_lookup \\ gs [OPTREL_def]
+    \\ rename1 ‘ref_rel _ _ y0’ \\ Cases_on ‘y0’ \\ gs [ref_rel_def]
+    \\ gvs [store_assign_def, store_lookup_def]
+    \\ rw [] \\ gs [v_rel_def]
+    \\ Q.REFINE_EXISTS_TAC
+      ‘<| refs := r1; ffi := f1; clock := s.clock;
+          next_type_stamp := nts1; next_exn_stamp := nes1;
+          eval_state := NONE |>’ \\ gs []
+    \\ Q.REFINE_EXISTS_TAC
+      ‘<| refs := r2; ffi := f2; clock := t.clock;
+          next_type_stamp := nts2; next_exn_stamp := nes2;
+          eval_state := NONE |>’ \\ gs []
+    \\ gs [state_rel_def, EL_LUPDATE]
+    \\ qx_gen_tac ‘n1’
+    \\ first_x_assum (qspec_then ‘n1’ assume_tac)
+    \\ rw [] \\ gs [ref_rel_def]
+    \\ qpat_x_assum ‘INJ ($' fr) _ _’ mp_tac \\ rw [INJ_DEF]
+    \\ qpat_x_assum ‘FLOOKUP fr _ = _’ mp_tac \\ rw [flookup_thm]
+    \\ qpat_x_assum ‘FLOOKUP fr _ = _’ mp_tac \\ rw [flookup_thm]
+    \\ gs [])
+  \\ Cases_on ‘op = Aupdate_unsafe’ \\ gs []
+  >- (
+    Cases_on ‘res’ \\ gvs [do_app_def, v_rel_def, OPTREL_def,
+                           CaseEqs ["list", "v", "option", "prod", "lit",
+                                    "store_v"]]
+    \\ rpt (irule_at Any SUBMAP_REFL) \\ gs []
+    \\ drule_all_then assume_tac state_rel_store_lookup \\ gs [OPTREL_def]
+    \\ rename1 ‘ref_rel _ _ y0’ \\ Cases_on ‘y0’ \\ gs [ref_rel_def]
+    \\ gvs [store_assign_def, store_lookup_def, store_v_same_type_def]
+    \\ rw [] \\ gs [v_rel_def]
+    \\ drule_then assume_tac LIST_REL_LENGTH \\ gs []
+    \\ Q.REFINE_EXISTS_TAC
+      ‘<| refs := r1; ffi := f1; clock := s.clock;
+          next_type_stamp := nts1; next_exn_stamp := nes1;
+          eval_state := NONE |>’ \\ gs []
+    \\ Q.REFINE_EXISTS_TAC
+      ‘<| refs := r2; ffi := f2; clock := t.clock;
+          next_type_stamp := nts2; next_exn_stamp := nes2;
+          eval_state := NONE |>’ \\ gs []
+    \\ gs [state_rel_def, EL_LUPDATE]
+    \\ qx_gen_tac ‘n1’
+    \\ first_x_assum (qspec_then ‘n1’ assume_tac)
+    \\ rw [] \\ gs [ref_rel_def]
+    \\ gvs [LIST_REL_EL_EQN, EL_LUPDATE]
+    \\ rw [] \\ gs []
+    \\ qpat_x_assum ‘INJ ($' fr) _ _’ mp_tac \\ rw [INJ_DEF]
+    \\ qpat_x_assum ‘FLOOKUP fr _ = _’ mp_tac \\ rw [flookup_thm]
+    \\ qpat_x_assum ‘FLOOKUP fr _ = _’ mp_tac \\ rw [flookup_thm]
+    \\ gs [])
+  \\ Cases_on ‘op = Asub_unsafe’ \\ gs []
+  >- (
+    Cases_on ‘res’ \\ gvs [do_app_def, v_rel_def, OPTREL_def,
+                           CaseEqs ["list", "v", "option", "prod", "lit",
+                                    "store_v"]]
+    \\ rpt (irule_at Any SUBMAP_REFL) \\ gs []
+    \\ drule_all_then assume_tac state_rel_store_lookup \\ gs [OPTREL_def]
+    \\ rename1 ‘ref_rel _ _ y0’ \\ Cases_on ‘y0’ \\ gs [ref_rel_def]
+    \\ rw [] \\ gs []
+    \\ gs [LIST_REL_EL_EQN]
+    \\ first_assum (irule_at Any) \\ gs [])
+  \\ Cases_on ‘op = Aupdate’ \\ gs []
+  >- (
+    Cases_on ‘res’ \\ gvs [do_app_def, v_rel_def, OPTREL_def,
+                           CaseEqs ["list", "v", "option", "prod", "lit",
+                                    "store_v"]]
+    \\ rpt (irule_at Any SUBMAP_REFL) \\ gs []
+    \\ drule_all_then assume_tac state_rel_store_lookup \\ gs [OPTREL_def]
+    \\ rename1 ‘ref_rel _ _ y0’ \\ Cases_on ‘y0’ \\ gs [ref_rel_def]
+    \\ gvs [store_assign_def, store_lookup_def, store_v_same_type_def]
+    \\ rw [] \\ gs [v_rel_def]
+    \\ drule_then assume_tac LIST_REL_LENGTH \\ gvs []
+    \\ Q.REFINE_EXISTS_TAC
+      ‘<| refs := r1; ffi := f1; clock := s.clock;
+          next_type_stamp := nts1; next_exn_stamp := nes1;
+          eval_state := NONE |>’ \\ gs []
+    \\ Q.REFINE_EXISTS_TAC
+      ‘<| refs := r2; ffi := f2; clock := t.clock;
+          next_type_stamp := nts2; next_exn_stamp := nes2;
+          eval_state := NONE |>’ \\ gs []
+    \\ gs [state_rel_def, EL_LUPDATE, sub_exn_v_def, v_rel_def, stamp_rel_cases,
+           subscript_stamp_def]
+    \\ qx_gen_tac ‘n1’
+    \\ first_x_assum (qspec_then ‘n1’ assume_tac)
+    \\ rw [] \\ gs [ref_rel_def]
+    \\ gvs [LIST_REL_EL_EQN, EL_LUPDATE]
+    \\ rw [] \\ gs []
+    \\ qpat_x_assum ‘INJ ($' fr) _ _’ mp_tac \\ rw [INJ_DEF]
+    \\ qpat_x_assum ‘FLOOKUP fr _ = _’ mp_tac \\ rw [flookup_thm]
+    \\ qpat_x_assum ‘FLOOKUP fr _ = _’ mp_tac \\ rw [flookup_thm]
+    \\ gs [])
+  \\ Cases_on ‘op = Alength’ \\ gs []
+  >- (
+    Cases_on ‘res’ \\ gvs [do_app_def, v_rel_def, OPTREL_def,
+                           CaseEqs ["list", "v", "option", "prod", "lit",
+                                    "store_v"]]
+    \\ rpt (irule_at Any SUBMAP_REFL) \\ gs []
+    \\ drule_all_then assume_tac state_rel_store_lookup \\ gs [OPTREL_def]
+    \\ rename1 ‘ref_rel _ _ y0’ \\ Cases_on ‘y0’ \\ gs [ref_rel_def, v_rel_def]
+    \\ gvs [store_assign_def, store_lookup_def, store_v_same_type_def]
+    \\ drule_then assume_tac LIST_REL_LENGTH \\ gvs []
+    \\ Q.REFINE_EXISTS_TAC
+      ‘<| refs := r1; ffi := f1; clock := s.clock;
+          next_type_stamp := nts1; next_exn_stamp := nes1;
+          eval_state := NONE |>’ \\ gs []
+    \\ Q.REFINE_EXISTS_TAC
+      ‘<| refs := r2; ffi := f2; clock := t.clock;
+          next_type_stamp := nts2; next_exn_stamp := nes2;
+          eval_state := NONE |>’ \\ gs []
+    \\ gs [state_rel_def])
+  \\ Cases_on ‘op = Asub’ \\ gs []
+  >- (
+    Cases_on ‘res’ \\ gvs [do_app_def, v_rel_def, OPTREL_def,
+                           CaseEqs ["list", "v", "option", "prod", "lit",
+                                    "store_v"]]
+    \\ rpt (irule_at Any SUBMAP_REFL) \\ gs []
+    \\ drule_all_then assume_tac state_rel_store_lookup \\ gs [OPTREL_def]
+    \\ rename1 ‘ref_rel _ _ y0’ \\ Cases_on ‘y0’ \\ gs [ref_rel_def]
+    \\ rw [] \\ gs []
+    \\ gvs [LIST_REL_EL_EQN]
+    \\ gs [state_rel_def, sub_exn_v_def, v_rel_def, stamp_rel_cases,
+           subscript_stamp_def]
+    \\ Q.REFINE_EXISTS_TAC
+      ‘<| refs := r1; ffi := f1; clock := s.clock;
+          next_type_stamp := nts1; next_exn_stamp := nes1;
+          eval_state := NONE |>’ \\ gs []
+    \\ Q.REFINE_EXISTS_TAC
+      ‘<| refs := r2; ffi := f2; clock := t.clock;
+          next_type_stamp := nts2; next_exn_stamp := nes2;
+          eval_state := NONE |>’ \\ gs [])
+  \\ Cases_on ‘op = AallocEmpty’ \\ gs []
+  >- (
+    Cases_on ‘res’ \\ gvs [do_app_def, v_rel_def, OPTREL_def,
+                           CaseEqs ["list", "v", "option", "prod", "lit",
+                                    "store_v"]]
+    \\ TRY (rpt (irule_at Any SUBMAP_REFL) \\ gs [] \\ NO_TAC)
+    \\ rpt (pairarg_tac \\ gs []) \\ gvs []
+    \\ gvs [store_alloc_def, v_rel_def, PULL_EXISTS]
+    \\ qexists_tac ‘fr |+ (LENGTH s.refs,LENGTH t.refs)’
+    \\ irule_at Any SUBMAP_REFL
+    \\ irule_at Any SUBMAP_REFL
+    \\ Q.REFINE_EXISTS_TAC
+      ‘<| refs := r1; ffi := f1; clock := s.clock;
+          next_type_stamp := nts1; next_exn_stamp := nes1;
+          eval_state := NONE |>’ \\ gs []
+    \\ Q.REFINE_EXISTS_TAC
+      ‘<| refs := r2; ffi := f2; clock := t.clock;
+          next_type_stamp := nts2; next_exn_stamp := nes2;
+          eval_state := NONE |>’ \\ gs []
+    \\ gs [state_rel_def, FLOOKUP_UPDATE]
+    \\ conj_tac
+    >- (
+      qpat_x_assum ‘INJ ($' fr) _ _’ mp_tac
+      \\ simp [INJ_DEF, FAPPLY_FUPDATE_THM]
+      \\ rw [] \\ gs []
+      \\ first_x_assum drule \\ gs []
+      \\ first_x_assum drule \\ gs [])
+    \\ simp [count_add1]
+    \\ strip_tac
+    >- (
+      qx_gen_tac ‘n’
+      \\ rw [] \\ gs []
+      \\ first_x_assum drule \\ gs [])
+    \\ qx_gen_tac ‘n’
+    \\ first_x_assum (qspec_then ‘n’ assume_tac)
+    \\ rw [] \\ gs [EL_LENGTH_APPEND, ref_rel_def]
+    \\ gs [EL_APPEND_EQN]
+    \\ irule ref_rel_mono
+    \\ first_assum (irule_at Any) \\ rw []
+    \\ irule v_rel_update
+    \\ Q.LIST_EXISTS_TAC [‘fe’,‘fr’,‘ft’] \\ gs [])
+  \\ Cases_on ‘op = Aalloc’ \\ gs []
+  >- (
+    Cases_on ‘res’ \\ gvs [do_app_def, v_rel_def, OPTREL_def,
+                           CaseEqs ["list", "v", "option", "prod", "lit",
+                                    "store_v"]]
+    \\ TRY (rpt (irule_at Any SUBMAP_REFL) \\ gs [] \\ NO_TAC)
+    \\ rpt (pairarg_tac \\ gs []) \\ gvs []
+    \\ gvs [store_alloc_def, v_rel_def, PULL_EXISTS, CaseEqs ["bool", "option"],
+            v_rel_def, sub_exn_v_def, stamp_rel_cases, subscript_stamp_def]
+    >- (
+      rpt (irule_at Any SUBMAP_REFL \\ gs [])
+      \\ first_assum (irule_at Any)
+      \\ gs [state_rel_def])
+    \\ qexists_tac ‘fr |+ (LENGTH s.refs,LENGTH t.refs)’
+    \\ irule_at Any SUBMAP_REFL
+    \\ irule_at Any SUBMAP_REFL
+    \\ Q.REFINE_EXISTS_TAC
+      ‘<| refs := r1; ffi := f1; clock := s.clock;
+          next_type_stamp := nts1; next_exn_stamp := nes1;
+          eval_state := NONE |>’ \\ gs []
+    \\ Q.REFINE_EXISTS_TAC
+      ‘<| refs := r2; ffi := f2; clock := t.clock;
+          next_type_stamp := nts2; next_exn_stamp := nes2;
+          eval_state := NONE |>’ \\ gs []
+    \\ gs [state_rel_def, FLOOKUP_UPDATE, count_add1]
+    \\ conj_tac
+    >- (
+      qpat_x_assum ‘INJ ($' fr) _ _’ mp_tac
+      \\ simp [INJ_DEF, FAPPLY_FUPDATE_THM]
+      \\ rw [] \\ gs []
+      \\ first_x_assum drule \\ gs []
+      \\ first_x_assum drule \\ gs [])
+    \\ strip_tac
+    >- (
+      qx_gen_tac ‘n’
+      \\ rw [] \\ gs []
+      \\ first_x_assum drule \\ gs [])
+    \\ qx_gen_tac ‘n’
+    \\ first_x_assum (qspec_then ‘n’ assume_tac)
+    \\ rw [] \\ gs [EL_APPEND_EQN, ref_rel_def, LIST_REL_REPLICATE_same]
+    >- (
+      rw []
+      \\ irule v_rel_update
+      \\ first_assum (irule_at (Pat ‘v_rel’)) \\ gs [])
+    \\ irule ref_rel_mono
+    \\ first_assum (irule_at Any) \\ rw []
+    \\ irule v_rel_update
+    \\ first_assum (irule_at (Pat ‘v_rel’)) \\ gs [])
+  \\ Cases_on ‘op = Vlength’ \\ gs []
+  >- (
+    Cases_on ‘res’ \\ gvs [do_app_def, v_rel_def, OPTREL_def,
+                           CaseEqs ["list", "v", "option", "prod", "lit",
+                                    "store_v"]]
+    \\ rpt (irule_at Any SUBMAP_REFL) \\ gs []
+    \\ first_assum (irule_at Any)
+    \\ gs [LIST_REL_EL_EQN])
+  \\ Cases_on ‘op = Vsub’ \\ gs []
+  >- (
+    Cases_on ‘res’ \\ gvs [do_app_def, v_rel_def, OPTREL_def,
+                           CaseEqs ["list", "v", "option", "prod", "lit",
+                                    "store_v"]]
+    \\ rpt (irule_at Any SUBMAP_REFL) \\ gs []
+    \\ rw [] \\ gvs [CaseEqs ["bool", "option"]]
+    \\ gvs [store_alloc_def, v_rel_def, PULL_EXISTS, CaseEqs ["bool", "option"],
+            v_rel_def, sub_exn_v_def, stamp_rel_cases, subscript_stamp_def]
+    \\ first_assum (irule_at Any)
+    \\ gs [state_rel_def, LIST_REL_EL_EQN])
+  \\ Cases_on ‘op = VfromList’ \\ gs []
+  >- (
+    ‘FLOOKUP ft list_type_num = SOME list_type_num ∧
+     INJ ($' ft) (FDOM ft) (count t.next_type_stamp) ∧
+     list_type_num < t.next_type_stamp’
+      by (gs [state_rel_def]
+          \\ qpat_x_assum ‘INJ ($' ft) _ _’ mp_tac \\ rw [INJ_DEF]
+          \\ rpt (first_x_assum (qspec_then ‘list_type_num’ assume_tac))
+          \\ gs [flookup_thm])
+    \\ Cases_on ‘res’ \\ gvs [do_app_def, v_rel_def, OPTREL_def,
+                              CaseEqs ["list", "v", "option", "prod", "lit",
+                                       "store_v"]]
+    \\ rpt (irule_at Any SUBMAP_REFL) \\ gs []
+    \\ rename1 ‘v_rel _ _ _ x1 x2’
+    \\ ‘∃res. v_to_list x2 = res’ by gs []
+    \\ drule_all v_rel_v_to_list \\ rw [OPTREL_def]
+    \\ first_assum (irule_at Any) \\ gs [v_rel_def]
+    \\ first_assum (irule_at Any) \\ gs [])
+  \\ Cases_on ‘op = Strcat’ \\ gs []
+  >- (
+    ‘FLOOKUP ft list_type_num = SOME list_type_num ∧
+     INJ ($' ft) (FDOM ft) (count t.next_type_stamp) ∧
+     list_type_num < t.next_type_stamp’
+      by (gs [state_rel_def]
+          \\ qpat_x_assum ‘INJ ($' ft) _ _’ mp_tac \\ rw [INJ_DEF]
+          \\ rpt (first_x_assum (qspec_then ‘list_type_num’ assume_tac))
+          \\ gs [flookup_thm])
+    \\ Cases_on ‘res’ \\ gvs [do_app_def, v_rel_def, OPTREL_def,
+                              CaseEqs ["list", "v", "option", "prod", "lit",
+                                       "store_v"]]
+    \\ rpt (irule_at Any SUBMAP_REFL) \\ gs []
+    \\ rename1 ‘v_rel _ _ _ x1 x2’
+    \\ ‘∃res. v_to_list x2 = res’ by gs []
+    \\ drule_all v_rel_v_to_list \\ rw [OPTREL_def]
+    \\ gs [option_nchotomy]
+    \\ rename1 ‘LIST_REL _ y1 y2’
+    \\ ‘∃res. vs_to_string y2 = res’ by gs []
+    \\ drule_all v_rel_vs_to_string \\ rw []
+    \\ gs [v_rel_def]
+    \\ first_assum (irule_at Any)
+    \\ irule_at Any EQ_REFL \\ gs [])
+  \\ Cases_on ‘op = Strlen’ \\ gs []
+  >- (
+    Cases_on ‘res’ \\ gvs [do_app_def, v_rel_def, OPTREL_def,
+                           CaseEqs ["list", "v", "option", "prod", "lit",
+                                    "store_v"]]
+    \\ rpt (irule_at Any SUBMAP_REFL) \\ gs []
+    \\ first_assum (irule_at Any) \\ gs [])
+  \\ Cases_on ‘op = Strsub’ \\ gs []
+  >- (
+    Cases_on ‘res’ \\ gvs [do_app_def, v_rel_def, OPTREL_def,
+                           CaseEqs ["list", "v", "option", "prod", "lit",
+                                    "store_v"]]
+    \\ rpt (irule_at Any SUBMAP_REFL) \\ gs []
+    \\ rw [] \\ gvs []
+    \\ first_assum (irule_at Any) \\ gs []
+    \\ gs [v_rel_def, sub_exn_v_def, stamp_rel_cases, subscript_stamp_def,
+           state_rel_def])
+  \\ Cases_on ‘op = Explode’ \\ gs []
+  >- (
+    Cases_on ‘res’ \\ gvs [do_app_def, v_rel_def, OPTREL_def,
+                           CaseEqs ["list", "v", "option", "prod", "lit",
+                                    "store_v"]]
+    \\ rpt (irule_at Any SUBMAP_REFL) \\ gs []
+    \\ gs [v_rel_def]
+    \\ first_assum (irule_at Any) \\ gs []
+    \\ irule v_rel_list_to_v
+    \\ irule_at Any v_to_list_list_to_v
+    \\ irule_at Any v_to_list_list_to_v
+    \\ gs [state_rel_def, EVERY2_MAP, LIST_REL_EL_EQN, v_rel_def])
+  \\ Cases_on ‘op = Implode’ \\ gs []
+  >- (
+    ‘FLOOKUP ft list_type_num = SOME list_type_num ∧
+     INJ ($' ft) (FDOM ft) (count t.next_type_stamp) ∧
+     list_type_num < t.next_type_stamp’
+      by (gs [state_rel_def]
+          \\ qpat_x_assum ‘INJ ($' ft) _ _’ mp_tac \\ rw [INJ_DEF]
+          \\ rpt (first_x_assum (qspec_then ‘list_type_num’ assume_tac))
+          \\ gs [flookup_thm])
+    \\ Cases_on ‘res’ \\ gvs [do_app_def, v_rel_def, OPTREL_def,
+                              CaseEqs ["list", "v", "option", "prod", "lit",
+                                       "store_v"]]
+    \\ rpt (irule_at Any SUBMAP_REFL) \\ gs []
+    \\ rename1 ‘v_rel _ _ _ x1 x2’
+    \\ ‘∃res. v_to_char_list x2 = res’ by gs []
+    \\ drule_all v_rel_v_to_char_list \\ rw []
+    \\ first_assum (irule_at Any)
+    \\ gs [v_rel_def])
+  \\ Cases_on ‘∃opb. op = Chopb opb’ \\ gs []
+  >- (
+    Cases_on ‘res’ \\ gvs [do_app_def, v_rel_def, OPTREL_def,
+                           CaseEqs ["list", "v", "option", "prod", "lit",
+                                    "store_v"]]
+    \\ rpt (irule_at Any SUBMAP_REFL) \\ gs []
+    \\ first_assum (irule_at Any) \\ gs []
+    \\ gs [Boolv_def] \\ rw []
+    \\ gs [v_rel_def, stamp_rel_cases, state_rel_def])
+  \\ Cases_on ‘op = Chr’ \\ gs []
+  >- (
+    Cases_on ‘res’ \\ gvs [do_app_def, v_rel_def, OPTREL_def,
+                           CaseEqs ["list", "v", "option", "prod", "lit",
+                                    "store_v"]]
+    \\ rpt (irule_at Any SUBMAP_REFL) \\ gs []
+    \\ first_assum (irule_at Any) \\ gs []
+    \\ rw [] \\ gs [v_rel_def, chr_exn_v_def, stamp_rel_cases, chr_stamp_def,
+                    state_rel_def])
+  \\ Cases_on ‘op = Ord’ \\ gs []
+  >- (
+    Cases_on ‘res’ \\ gvs [do_app_def, v_rel_def, OPTREL_def,
+                           CaseEqs ["list", "v", "option", "prod", "lit",
+                                    "store_v"]]
+    \\ rpt (irule_at Any SUBMAP_REFL) \\ gs []
+    \\ first_assum (irule_at Any) \\ gs [])
+  \\ Cases_on ‘op = CopyAw8Aw8’ \\ gs []
+  >- (
+    Cases_on ‘res’ \\ gvs [do_app_def, v_rel_def, OPTREL_def,
+                           CaseEqs ["list", "v", "option", "prod", "lit",
+                                    "store_v"], PULL_EXISTS]
+    \\ rpt (irule_at Any SUBMAP_REFL \\ gs [])
+    \\ imp_res_tac state_rel_store_lookup \\ gs [OPTREL_def]
+    \\ rpt (rename [‘ref_rel _ (_ _) y0’] \\ Cases_on ‘y0’ \\ gvs [ref_rel_def])
+    \\ gvs [store_assign_def, store_lookup_def, copy_array_def,
+            v_rel_def, sub_exn_v_def, subscript_stamp_def, stamp_rel_cases]
+    >- (
+      first_assum (irule_at Any)
+      \\ gs [state_rel_def])
+    \\ Q.REFINE_EXISTS_TAC
+      ‘<| refs := r1; ffi := f1; clock := s.clock;
+          next_type_stamp := nts1; next_exn_stamp := nes1;
+          eval_state := NONE |>’ \\ gs []
+    \\ Q.REFINE_EXISTS_TAC
+      ‘<| refs := r2; ffi := f2; clock := t.clock;
+          next_type_stamp := nts2; next_exn_stamp := nes2;
+          eval_state := NONE |>’ \\ gs []
+    \\ gs [state_rel_def, EL_LUPDATE]
+    \\ qx_gen_tac ‘n1’
+    \\ first_x_assum (qspec_then ‘n1’ mp_tac)
+    \\ rw [] \\ gs [ref_rel_def]
+    \\ rw [] \\ gs [ref_rel_def]
+    \\ qpat_x_assum ‘INJ ($' fr) _ _’ mp_tac
+    \\ rpt (qpat_x_assum ‘FLOOKUP _ _ = _’ mp_tac)
+    \\ rw [flookup_thm, INJ_DEF] \\ gs [])
+  \\ Cases_on ‘op = CopyAw8Str’ \\ gs []
+  >- (
+    Cases_on ‘res’ \\ gvs [do_app_def, v_rel_def, OPTREL_def,
+                           CaseEqs ["list", "v", "option", "prod", "lit",
+                                    "store_v"], PULL_EXISTS]
+    \\ rpt (irule_at Any SUBMAP_REFL \\ gs [])
+    \\ imp_res_tac state_rel_store_lookup \\ gs [OPTREL_def]
+    \\ rpt (rename [‘ref_rel _ (_ _) y0’] \\ Cases_on ‘y0’ \\ gvs [ref_rel_def])
+    \\ gvs [store_assign_def, store_lookup_def, copy_array_def,
+            v_rel_def, sub_exn_v_def, subscript_stamp_def, stamp_rel_cases]
+    \\ Q.REFINE_EXISTS_TAC
+      ‘<| refs := r1; ffi := f1; clock := s.clock;
+          next_type_stamp := nts1; next_exn_stamp := nes1;
+          eval_state := NONE |>’ \\ gs []
+    \\ Q.REFINE_EXISTS_TAC
+      ‘<| refs := r2; ffi := f2; clock := t.clock;
+          next_type_stamp := nts2; next_exn_stamp := nes2;
+          eval_state := NONE |>’ \\ gs []
+    \\ gs [state_rel_def, EL_LUPDATE]
+    \\ rw [] \\ gs [ref_rel_def, v_rel_def, stamp_rel_cases])
+  \\ Cases_on ‘op = CopyStrAw8’ \\ gs []
+  >- (
+    Cases_on ‘res’ \\ gvs [do_app_def, v_rel_def, OPTREL_def,
+                           CaseEqs ["list", "v", "option", "prod", "lit",
+                                    "store_v"], PULL_EXISTS]
+    \\ rpt (irule_at Any SUBMAP_REFL \\ gs [])
+    \\ imp_res_tac state_rel_store_lookup \\ gs [OPTREL_def]
+    \\ rpt (rename [‘ref_rel _ (_ _) y0’] \\ Cases_on ‘y0’ \\ gvs [ref_rel_def])
+    \\ gvs [store_assign_def, store_lookup_def, copy_array_def,
+            v_rel_def, sub_exn_v_def, subscript_stamp_def, stamp_rel_cases]
+    \\ Q.REFINE_EXISTS_TAC
+      ‘<| refs := r1; ffi := f1; clock := s.clock;
+          next_type_stamp := nts1; next_exn_stamp := nes1;
+          eval_state := NONE |>’ \\ gs []
+    \\ Q.REFINE_EXISTS_TAC
+      ‘<| refs := r2; ffi := f2; clock := t.clock;
+          next_type_stamp := nts2; next_exn_stamp := nes2;
+          eval_state := NONE |>’ \\ gs []
+    \\ gs [state_rel_def, EL_LUPDATE]
+    \\ qx_gen_tac ‘n1’
+    \\ first_x_assum (qspec_then ‘n1’ mp_tac)
+    \\ rw [] \\ gs [ref_rel_def]
+    \\ rw [] \\ gs [ref_rel_def]
+    \\ qpat_x_assum ‘INJ ($' fr) _ _’ mp_tac
+    \\ rpt (qpat_x_assum ‘FLOOKUP _ _ = _’ mp_tac)
+    \\ rw [flookup_thm, INJ_DEF] \\ gs [])
+  \\ Cases_on ‘op = CopyStrStr’ \\ gs []
+  >- (
+    Cases_on ‘res’ \\ gvs [do_app_def, v_rel_def, OPTREL_def,
+                           CaseEqs ["list", "v", "option", "prod", "lit",
+                                    "store_v"], PULL_EXISTS]
+    \\ rpt (irule_at Any SUBMAP_REFL \\ gs [])
+    \\ imp_res_tac state_rel_store_lookup \\ gs [OPTREL_def]
+    \\ rpt (rename [‘ref_rel _ (_ _) y0’] \\ Cases_on ‘y0’ \\ gvs [ref_rel_def])
+    \\ gvs [store_assign_def, store_lookup_def, copy_array_def,
+            v_rel_def, sub_exn_v_def, subscript_stamp_def, stamp_rel_cases]
+    \\ Q.REFINE_EXISTS_TAC
+      ‘<| refs := r1; ffi := f1; clock := s.clock;
+          next_type_stamp := nts1; next_exn_stamp := nes1;
+          eval_state := NONE |>’ \\ gs []
+    \\ Q.REFINE_EXISTS_TAC
+      ‘<| refs := r2; ffi := f2; clock := t.clock;
+          next_type_stamp := nts2; next_exn_stamp := nes2;
+          eval_state := NONE |>’ \\ gs []
+    \\ gs [state_rel_def, EL_LUPDATE]
+    \\ rw [] \\ gs [ref_rel_def, v_rel_def, stamp_rel_cases])
+  \\ Cases_on ‘∃n. op = WordToInt n’ \\ gs []
+  >- (
+    Cases_on ‘res’ \\ gvs [do_app_def, v_rel_def, OPTREL_def,
+                           CaseEqs ["list", "v", "option", "prod", "lit",
+                                    "store_v", "word_size"], PULL_EXISTS]
+    \\ rpt (irule_at Any SUBMAP_REFL \\ gs [])
+    \\ first_assum (irule_at Any) \\ gs [])
+  \\ Cases_on ‘∃n. op = WordFromInt n’ \\ gs []
+  >- (
+    Cases_on ‘res’ \\ gvs [do_app_def, v_rel_def, OPTREL_def,
+                           CaseEqs ["list", "v", "option", "prod", "lit",
+                                    "store_v", "word_size"], PULL_EXISTS]
+    \\ rpt (irule_at Any SUBMAP_REFL \\ gs [])
+    \\ first_assum (irule_at Any) \\ gs [])
+  \\ Cases_on ‘op = Aw8update’ \\ gs []
+  >- (
+    Cases_on ‘res’ \\ gvs [do_app_def, v_rel_def, OPTREL_def,
+                           CaseEqs ["list", "v", "option", "prod", "lit",
+                                    "store_v"]]
+    \\ rpt (irule_at Any SUBMAP_REFL) \\ gs []
+    \\ drule_all_then assume_tac state_rel_store_lookup \\ gs [OPTREL_def]
+    \\ rename1 ‘ref_rel _ _ y0’ \\ Cases_on ‘y0’ \\ gs [ref_rel_def]
+    \\ gvs [store_assign_def, store_lookup_def]
+    \\ rw [] \\ gvs [v_rel_def, sub_exn_v_def, subscript_stamp_def,
+                     stamp_rel_cases]
+    \\ Q.REFINE_EXISTS_TAC
+      ‘<| refs := r1; ffi := f1; clock := s.clock;
+          next_type_stamp := nts1; next_exn_stamp := nes1;
+          eval_state := NONE |>’ \\ gs []
+    \\ Q.REFINE_EXISTS_TAC
+      ‘<| refs := r2; ffi := f2; clock := t.clock;
+          next_type_stamp := nts2; next_exn_stamp := nes2;
+          eval_state := NONE |>’ \\ gs []
+    \\ gs [state_rel_def, EL_LUPDATE]
+    \\ qx_gen_tac ‘n1’
+    \\ first_x_assum (qspec_then ‘n1’ assume_tac)
+    \\ rw [] \\ gs [ref_rel_def]
+    \\ rw [] \\ gs [ref_rel_def]
+    \\ qpat_x_assum ‘INJ ($' fr) _ _’ mp_tac \\ rw [INJ_DEF]
+    \\ qpat_x_assum ‘FLOOKUP fr _ = _’ mp_tac \\ rw [flookup_thm]
+    \\ qpat_x_assum ‘FLOOKUP fr _ = _’ mp_tac \\ rw [flookup_thm]
+    \\ gs [])
+  \\ Cases_on ‘op = Aw8sub’ \\ gs []
+  >- (
+    Cases_on ‘res’ \\ gvs [do_app_def, v_rel_def, OPTREL_def,
+                           CaseEqs ["list", "v", "option", "prod", "lit",
+                                    "store_v"]]
+    \\ rpt (irule_at Any SUBMAP_REFL) \\ gs []
+    \\ drule_all_then assume_tac state_rel_store_lookup \\ gs [OPTREL_def]
+    \\ rename1 ‘ref_rel _ _ y0’ \\ Cases_on ‘y0’ \\ gs [ref_rel_def]
+    \\ rw [] \\ gvs [LIST_REL_EL_EQN, v_rel_def, sub_exn_v_def,
+                     subscript_stamp_def, stamp_rel_cases]
+    \\ first_assum (irule_at Any) \\ gs [state_rel_def])
+  \\ Cases_on ‘op = Aw8length’ \\ gs []
+  >- (
+    Cases_on ‘res’ \\ gvs [do_app_def, v_rel_def, OPTREL_def,
+                           CaseEqs ["list", "v", "option", "prod", "lit",
+                                    "store_v"]]
+    \\ rpt (irule_at Any SUBMAP_REFL) \\ gs []
+    \\ drule_all_then assume_tac state_rel_store_lookup \\ gs [OPTREL_def]
+    \\ rename1 ‘ref_rel _ _ y0’ \\ Cases_on ‘y0’ \\ gs [ref_rel_def]
+    \\ rw [] \\ gvs [LIST_REL_EL_EQN, v_rel_def]
+    \\ first_assum (irule_at Any) \\ gs [])
+  \\ Cases_on ‘op = Aw8alloc’ \\ gs []
+  >- (
+    Cases_on ‘res’ \\ gvs [do_app_def, v_rel_def, OPTREL_def,
+                           CaseEqs ["list", "v", "option", "prod", "lit",
+                                    "store_v"]]
+    \\ TRY (rpt (irule_at Any SUBMAP_REFL) \\ gs [] \\ NO_TAC)
+    \\ rpt (pairarg_tac \\ gs []) \\ gvs []
+    \\ gvs [store_alloc_def, v_rel_def, PULL_EXISTS, CaseEqs ["bool", "option"],
+            v_rel_def, sub_exn_v_def, stamp_rel_cases, subscript_stamp_def]
+    >- (
+      rpt (irule_at Any SUBMAP_REFL \\ gs [])
+      \\ first_assum (irule_at Any)
+      \\ gs [state_rel_def])
+    \\ qexists_tac ‘fr |+ (LENGTH s.refs,LENGTH t.refs)’
+    \\ irule_at Any SUBMAP_REFL
+    \\ irule_at Any SUBMAP_REFL
+    \\ Q.REFINE_EXISTS_TAC
+      ‘<| refs := r1; ffi := f1; clock := s.clock;
+          next_type_stamp := nts1; next_exn_stamp := nes1;
+          eval_state := NONE |>’ \\ gs []
+    \\ Q.REFINE_EXISTS_TAC
+      ‘<| refs := r2; ffi := f2; clock := t.clock;
+          next_type_stamp := nts2; next_exn_stamp := nes2;
+          eval_state := NONE |>’ \\ gs []
+    \\ gs [state_rel_def, FLOOKUP_UPDATE, count_add1]
+    \\ conj_tac
+    >- (
+      qpat_x_assum ‘INJ ($' fr) _ _’ mp_tac
+      \\ simp [INJ_DEF, FAPPLY_FUPDATE_THM]
+      \\ rw [] \\ gs []
+      \\ first_x_assum drule \\ gs []
+      \\ first_x_assum drule \\ gs [])
+    \\ strip_tac
+    >- (
+      qx_gen_tac ‘n’
+      \\ rw [] \\ gs []
+      \\ first_x_assum drule \\ gs [])
+    \\ qx_gen_tac ‘n’
+    \\ first_x_assum (qspec_then ‘n’ assume_tac)
+    \\ rw [] \\ gs [EL_APPEND_EQN, ref_rel_def, LIST_REL_REPLICATE_same]
+    \\ irule ref_rel_mono
+    \\ first_assum (irule_at Any) \\ rw []
+    \\ irule v_rel_update
+    \\ first_assum (irule_at (Pat ‘v_rel’)) \\ gs [])
+  \\ Cases_on ‘∃top. op = FP_top top’ \\ gs []
+  >- (
+    Cases_on ‘res’ \\ gvs [do_app_def, v_rel_def, OPTREL_def,
+                           CaseEqs ["list", "v", "option", "prod", "lit",
+                                    "store_v"]]
+    \\ rpt (irule_at Any SUBMAP_REFL) \\ gs []
+    \\ first_assum (irule_at Any) \\ gs [])
+  \\ Cases_on ‘∃bop. op = FP_bop bop’ \\ gs []
+  >- (
+    Cases_on ‘res’ \\ gvs [do_app_def, v_rel_def, OPTREL_def,
+                           CaseEqs ["list", "v", "option", "prod", "lit",
+                                    "store_v"]]
+    \\ rpt (irule_at Any SUBMAP_REFL) \\ gs []
+    \\ first_assum (irule_at Any) \\ gs [])
+  \\ Cases_on ‘∃uop. op = FP_uop uop’ \\ gs []
+  >- (
+    Cases_on ‘res’ \\ gvs [do_app_def, v_rel_def, OPTREL_def,
+                           CaseEqs ["list", "v", "option", "prod", "lit",
+                                    "store_v"]]
+    \\ rpt (irule_at Any SUBMAP_REFL) \\ gs []
+    \\ first_assum (irule_at Any) \\ gs [])
+  \\ Cases_on ‘∃cmp. op = FP_cmp cmp’ \\ gs []
+  >- (
+    Cases_on ‘res’ \\ gvs [do_app_def, v_rel_def, OPTREL_def,
+                           CaseEqs ["list", "v", "option", "prod", "lit",
+                                    "store_v"]]
+    \\ rpt (irule_at Any SUBMAP_REFL) \\ gs []
+    \\ first_assum (irule_at Any) \\ gs []
+    \\ gs [Boolv_def] \\ rw [v_rel_def, stamp_rel_cases]
+    \\ gs [state_rel_def])
+  \\ Cases_on ‘∃opn. op = Opn opn’ \\ gs []
+  >- (
+    Cases_on ‘res’ \\ gvs [do_app_def, v_rel_def, OPTREL_def,
+                           CaseEqs ["list", "v", "option", "prod", "lit",
+                                    "store_v"]]
+    \\ rpt (irule_at Any SUBMAP_REFL) \\ gs []
+    \\ rw [] \\ gvs []
+    \\ first_assum (irule_at Any) \\ gs []
+    \\ gs [v_rel_def, div_exn_v_def, div_stamp_def, stamp_rel_cases,
+           state_rel_def])
+  \\ Cases_on ‘∃opb. op = Opb opb’ \\ gs []
+  >- (
+    Cases_on ‘res’ \\ gvs [do_app_def, v_rel_def, OPTREL_def,
+                           CaseEqs ["list", "v", "option", "prod", "lit",
+                                    "store_v"]]
+    \\ rpt (irule_at Any SUBMAP_REFL) \\ gs []
+    \\ rw [] \\ gvs []
+    \\ first_assum (irule_at Any) \\ gs []
+    \\ gs [Boolv_def] \\ rw [v_rel_def, stamp_rel_cases]
+    \\ gs [state_rel_def])
+  \\ Cases_on ‘∃sz opw. op = Opw sz opw’ \\ gs []
+  >- (
+    Cases_on ‘res’ \\ gvs [do_app_def, v_rel_def, OPTREL_def,
+                           CaseEqs ["list", "v", "option", "prod", "lit",
+                                    "store_v", "word_size"]]
+    \\ rpt (irule_at Any SUBMAP_REFL) \\ gs []
+    \\ first_assum (irule_at Any) \\ gs [])
+  \\ Cases_on ‘∃sz sh n. op = Shift sz sh n’ \\ gs []
+  >- (
+    Cases_on ‘res’ \\ gvs [do_app_def, v_rel_def, OPTREL_def,
+                           CaseEqs ["list", "v", "option", "prod", "lit",
+                                    "store_v", "word_size"]]
+    \\ rpt (irule_at Any SUBMAP_REFL) \\ gs []
+    \\ first_assum (irule_at Any) \\ gs [])
+  \\ Cases_on ‘op = Equality’ \\ gs []
+  >- (
+    Cases_on ‘res’ \\ gvs [do_app_def, v_rel_def, OPTREL_def,
+                           CaseEqs ["list", "v", "option", "prod", "lit",
+                                    "store_v", "word_size"]]
+    \\ rpt (irule_at Any SUBMAP_REFL) \\ gs []
+    \\ gs [CaseEqs ["eq_result"], EXISTS_PROD, PULL_EXISTS]
+    \\ gs [state_rel_def]
+    \\ rename1 ‘v_rel _ _ _ x1 x2’ \\ rename1 ‘v_rel _ _ _ y1 y2’
+    >- (
+      qpat_assum ‘do_eq _ _ = _’ (SUBST1_TAC o SYM)
+      \\ once_rewrite_tac [EQ_SYM_EQ]
+      \\ irule (CONJUNCT1 v_rel_do_eq)
+      \\ first_assum (irule_at Any) \\ gs []
+      \\ first_assum (irule_at Any) \\ gs []
+      \\ first_assum (irule_at Any) \\ gs []
+      \\ first_assum (irule_at Any) \\ gs [])
+    \\ qexists_tac ‘b’
+    \\ qpat_assum ‘do_eq _ _ = _’ (SUBST1_TAC o SYM)
+    \\ simp_tac std_ss [Once EQ_SYM_EQ]
+    \\ irule_at Any (CONJUNCT1 v_rel_do_eq) \\ gvs []
+    \\ first_assum (irule_at (Pat ‘v_rel’)) \\ gs []
+    \\ Q.REFINE_EXISTS_TAC
+      ‘<| refs := r1; ffi := f1; clock := s.clock;
+          next_type_stamp := nts1; next_exn_stamp := nes1;
+          eval_state := NONE |>’ \\ gs []
+    \\ Q.REFINE_EXISTS_TAC
+      ‘<| refs := r2; ffi := f2; clock := t.clock;
+          next_type_stamp := nts2; next_exn_stamp := nes2;
+          eval_state := NONE |>’ \\ gs []
+    \\ rw [Boolv_def]
+    \\ gs [v_rel_def, stamp_rel_cases, SF SFY_ss])
+  \\ Cases_on ‘op = Opderef’ \\ gs []
+  >- (
+    Cases_on ‘res’ \\ gvs [do_app_def, v_rel_def, OPTREL_def,
+                           CaseEqs ["list", "v", "option", "prod", "lit",
+                                    "store_v"]]
+    \\ rpt (irule_at Any SUBMAP_REFL) \\ gs []
+    \\ drule_all_then assume_tac state_rel_store_lookup \\ gs [OPTREL_def]
+    \\ rename1 ‘ref_rel _ _ y0’ \\ Cases_on ‘y0’ \\ gs [ref_rel_def]
+    \\ first_assum (irule_at Any) \\ gs [])
+  \\ Cases_on ‘op = Opassign’ \\ gs []
+  >- (
+    Cases_on ‘res’ \\ gvs [do_app_def, v_rel_def, OPTREL_def,
+                           CaseEqs ["list", "v", "option", "prod", "lit",
+                                    "store_v"]]
+    \\ rpt (irule_at Any SUBMAP_REFL) \\ gs [v_rel_def]
+    \\ rename1 ‘v_rel fr ft fe v w’
+    \\ ‘ref_rel (v_rel fr ft fe) (Refv v) (Refv w)’
+      by gs [ref_rel_def]
+    \\ drule_all state_rel_store_assign \\ rw [OPTREL_def]
+    \\ first_assum (irule_at Any) \\ gs [])
+  \\ Cases_on ‘op = Opref’ \\ gs []
+  >- (
+    Cases_on ‘res’ \\ gvs [do_app_def, v_rel_def, OPTREL_def,
+                           CaseEqs ["list", "v", "option", "prod", "lit",
+                                    "store_v"]]
+    \\ TRY (rpt (irule_at Any SUBMAP_REFL) \\ gs [] \\ NO_TAC)
+    \\ rpt (pairarg_tac \\ gs []) \\ gvs []
+    \\ gvs [store_alloc_def, v_rel_def]
+    \\ qexists_tac ‘fr |+ (LENGTH s.refs,LENGTH t.refs)’
+    \\ irule_at Any SUBMAP_REFL
+    \\ irule_at Any SUBMAP_REFL
+    \\ Q.REFINE_EXISTS_TAC
+      ‘<| refs := r1; ffi := f1; clock := s.clock;
+          next_type_stamp := nts1; next_exn_stamp := nes1;
+          eval_state := NONE |>’ \\ gs []
+    \\ Q.REFINE_EXISTS_TAC
+      ‘<| refs := r2; ffi := f2; clock := t.clock;
+          next_type_stamp := nts2; next_exn_stamp := nes2;
+          eval_state := NONE |>’ \\ gs []
+    \\ gs [state_rel_def, FLOOKUP_UPDATE, count_add1]
+    \\ conj_tac
+    >- (
+      qpat_x_assum ‘INJ ($' fr) _ _’ mp_tac
+      \\ rw [INJ_DEF, FAPPLY_FUPDATE_THM]
+      \\ rw [] \\ gs []
+      \\ first_x_assum drule \\ gs []
+      \\ first_x_assum drule \\ gs [])
+    \\ conj_tac
+    >- (
+      qx_gen_tac ‘n1’
+      \\ first_x_assum (qspec_then ‘n1’ assume_tac)
+      \\ rw [] \\ gs []
+      \\ first_x_assum drule \\ gs [])
+    \\ qx_gen_tac ‘n1’
+    \\ first_x_assum (qspec_then ‘n1’ assume_tac)
+    \\ rw [] \\ gs [EL_LENGTH_APPEND, ref_rel_def, EL_APPEND_EQN]
+    >- (
+      irule v_rel_update
+      \\ first_assum (irule_at (Pat ‘v_rel’))
+      \\ gs [])
+    \\ irule ref_rel_mono
+    \\ first_assum (irule_at Any) \\ rw []
+    \\ irule v_rel_update
+    \\ first_assum (irule_at (Pat ‘v_rel’))
+    \\ gs [])
+  \\ Cases_on ‘op’ \\ gs [] *)
+QED
+
+Theorem do_app_update = SIMP_RULE (srw_ss()) [LET_THM] do_app_update;
+
+Theorem evaluate_ok_Op:
+  op ≠ Opapp ∧ op ≠ Eval ⇒ ^(get_goal "App")
+Proof
+  rw [evaluate_def]
+  \\ gvs [CaseEqs ["prod", "result", "option"]]
+  \\ dxrule_then assume_tac (iffRL EVERY_REVERSE)
+  \\ drule_all_then assume_tac do_app_update \\ gs []
+  \\ gs [env_ok_def]
+  \\ drule_then assume_tac (CONJUNCT1 evaluate_next_type_stamp_mono)
+  \\ drule_then assume_tac (CONJUNCT1 evaluate_next_exn_stamp_mono)
+  \\ drule_then assume_tac (CONJUNCT1 evaluate_refs_length_mono)
+  \\ drule_then assume_tac do_app_refs_length
+  \\ irule env_rel_update
+  \\ first_assum (irule_at Any)
+  \\ gs [FUN_FMAP_SUBMAP_SUBSET, COUNT_MONO]
+QED
+
+Theorem do_opapp_cases[local] = semanticPrimitivesPropsTheory.do_opapp_cases;
+
+Theorem do_opapp_update:
+  do_opapp vs = SOME (env, x) ∧
+  EVERY (v_ok s) vs ∧
+  state_ok s ⇒
+    env_ok s env
+Proof
+  rw [do_opapp_cases] \\ gs [v_ok_thm, env_ok_def]
+  \\ gs [semanticPrimitivesPropsTheory.find_recfun_ALOOKUP, v_ok_def]
+  >- (
+    irule_at Any env_rel_nsBind \\ gs [])
+  \\ gs [env_rel_def, semanticPrimitivesPropsTheory.build_rec_env_merge]
+  \\ irule nsAll2_nsBind \\ gs []
+  \\ irule nsAll2_nsAppend \\ gs []
+  \\ irule nsAll2_alist_to_ns \\ gs []
+  \\ gs [EVERY2_MAP, LAMBDA_PROD, v_rel_def, env_rel_def]
+  \\ rw [ELIM_UNCURRY, LIST_REL_EL_EQN]
+QED
+
+Theorem evaluate_ok_Opapp:
+  op = Opapp ⇒ ^(get_goal "App")
+Proof
+  simp [evaluate_def]
+  \\ strip_tac
+  \\ strip_tac
+  \\ rpt gen_tac
+  \\ strip_tac
+  \\ qpat_x_assum ‘_ = (t,res)’ mp_tac
+  \\ TOP_CASE_TAC \\ rfs []
+  \\ reverse TOP_CASE_TAC \\ rfs []
+  >- (
+    rw [] \\ gs [])
+  \\ TOP_CASE_TAC \\ gs []
+  \\ TOP_CASE_TAC \\ gs []
+  \\ IF_CASES_TAC \\ gs []
+  >- (
+    rw [] \\ gs [])
+  \\ strip_tac
+  \\ rename1 ‘evaluate (dec_clock s1) env1’
+  \\ ‘state_ok (dec_clock s1)’
+    by (qpat_x_assum ‘state_ok s1’ mp_tac
+        \\ rw [state_ok_def, dec_clock_def, state_rel_def]
+        \\ gs [])
+  \\ dxrule_then assume_tac (iffRL EVERY_REVERSE)
+  \\ drule_all_then assume_tac do_opapp_update
+  \\ ‘env_ok (dec_clock s1) env1’
+    by gs [env_ok_def, dec_clock_def]
+  \\ first_x_assum (drule_all_then strip_assume_tac) \\ gs []
+  \\ drule_then assume_tac (CONJUNCT1 evaluate_next_type_stamp_mono)
+  \\ drule_then assume_tac (CONJUNCT1 evaluate_next_exn_stamp_mono)
+  \\ dxrule_then assume_tac (CONJUNCT1 evaluate_refs_length_mono)
+  \\ drule_then assume_tac (CONJUNCT1 evaluate_next_type_stamp_mono)
+  \\ drule_then assume_tac (CONJUNCT1 evaluate_next_exn_stamp_mono)
+  \\ drule_then assume_tac (CONJUNCT1 evaluate_refs_length_mono)
+  \\ gs [dec_clock_def, env_ok_def]
+  \\ irule env_rel_update
+  \\ first_assum (irule_at Any)
+  \\ gs [FUN_FMAP_SUBMAP_SUBSET, COUNT_MONO]
+QED
+
+Theorem evaluate_ok_App:
+  ^(get_goal "App")
+Proof
+  Cases_on ‘op = Opapp’ >- (match_mp_tac evaluate_ok_Opapp \\ gs [])
+  \\ Cases_on ‘op = Eval’ >- (match_mp_tac evaluate_ok_Eval \\ gs [])
+  \\ match_mp_tac evaluate_ok_Op \\ gs []
+QED
+
+Theorem v_ok_Boolv[simp]:
+  state_ok s ⇒ v_ok s (Boolv b)
+Proof
+  rw [Boolv_def, state_ok_def, v_ok_thm, stamp_ok_def, stamp_rel_cases,
+      FLOOKUP_FUN_FMAP, state_rel_def]
+QED
+
+Theorem v_ok_do_log:
+  state_ok s ∧
+  v_ok s v ∧
+  do_log lop v x = SOME (Val w) ⇒ v_ok s w
+Proof
+  rw [] \\ gs []
+  \\ gs [do_log_def, CaseEq "bool"]
+QED
+
+Theorem evaluate_ok_Log:
+  ^(get_goal "Log")
+Proof
+  rw [evaluate_def]
+  \\ gvs [CaseEqs ["option", "prod", "result", "bool", "exp_or_val"]]
+  \\ drule_then strip_assume_tac evaluate_sing \\ gvs []
+  \\ drule_all_then assume_tac v_ok_do_log \\ gs []
+QED
+
+Theorem evaluate_ok_If:
+  ^(get_goal "If")
+Proof
+  rw [evaluate_def]
+  \\ gvs [CaseEqs ["option", "prod", "result", "bool", "exp_or_val"]]
+QED
+
+Theorem v_ok_bind_exn[simp]:
+  state_ok s ⇒ v_ok s bind_exn_v
+Proof
+  rw [state_ok_def, state_rel_def, v_ok_thm, stamp_ok_def, stamp_rel_cases,
+      bind_exn_v_def, bind_stamp_def]
+QED
+
+Theorem evaluate_ok_Mat:
+  ^(get_goal "Mat")
+Proof
+  simp [evaluate_def]
+  \\ strip_tac
+  \\ rpt gen_tac
+  \\ strip_tac
+  \\ qpat_x_assum ‘_ = (t,res)’ mp_tac
+  \\ TOP_CASE_TAC \\ rfs []
+  \\ reverse TOP_CASE_TAC \\ rfs []
+  >- (
+    rw [] \\ gs [])
+  \\ IF_CASES_TAC \\ gs []
+  \\ strip_tac
+  \\ drule_then strip_assume_tac evaluate_sing \\ gvs []
+QED
+
+Theorem evaluate_ok_Let:
+  ^(get_goal "Let")
+Proof
+  rw [evaluate_def]
+  \\ gvs [CaseEqs ["option", "prod", "result", "bool"]]
+  \\ imp_res_tac evaluate_sing \\ gvs []
+  \\ drule_all_then assume_tac evaluate_env_ok_mono
+  \\ rename1 ‘env_ok st1 (env with v := nsOptBind xo v1 env.v)’
+  \\ ‘env_ok st1 (env with v := nsOptBind xo v1 env.v)’
+    by (Cases_on ‘xo’ \\ gs [namespaceTheory.nsOptBind_def, env_rel_def,
+                           env_ok_def]
+        \\ irule nsAll2_nsBind \\ gs [] \\ gs [GSYM v_ok_def])
+  \\ drule_all_then assume_tac evaluate_env_ok_mono \\ gs []
+  \\ gs [env_ok_def]
+  \\ drule_then assume_tac (CONJUNCT1 evaluate_next_type_stamp_mono)
+  \\ drule_then assume_tac (CONJUNCT1 evaluate_next_exn_stamp_mono)
+  \\ drule_then assume_tac (CONJUNCT1 evaluate_refs_length_mono)
+  \\ irule env_rel_update
+  \\ first_assum (irule_at Any)
+  \\ gs [FUN_FMAP_SUBMAP_SUBSET, COUNT_MONO]
+QED
+
+Theorem evaluate_ok_Letrec:
+  ^(get_goal "Letrec")
+Proof
+  rw [evaluate_def] \\ gs [SF SFY_ss]
+  \\ rename1 ‘env_ok st (env with v := build_rec_env funs env env.v)’
+  \\ ‘env_ok st (env with v := build_rec_env funs env env.v)’
+    by (gs [env_rel_def, semanticPrimitivesPropsTheory.build_rec_env_merge,
+            env_ok_def]
+        \\ irule nsAll2_nsAppend \\ gs []
+        \\ irule nsAll2_alist_to_ns
+        \\ rw [EVERY2_MAP, LAMBDA_PROD, LIST_REL_EL_EQN]
+        \\ simp [ELIM_UNCURRY, v_rel_def, env_rel_def])
+  \\ drule_all_then assume_tac evaluate_env_ok_mono \\ gs []
+  \\ gs [env_ok_def]
+  \\ drule_then assume_tac (CONJUNCT1 evaluate_next_type_stamp_mono)
+  \\ drule_then assume_tac (CONJUNCT1 evaluate_next_exn_stamp_mono)
+  \\ drule_then assume_tac (CONJUNCT1 evaluate_refs_length_mono)
+  \\ irule env_rel_update
+  \\ first_assum (irule_at Any)
+  \\ gs [FUN_FMAP_SUBMAP_SUBSET, COUNT_MONO]
+QED
+
+Theorem evaluate_ok_Tannot:
+  ^(get_goal "Tannot")
+Proof
+  rw [evaluate_def]
+QED
+
+Theorem evaluate_ok_Lannot:
+  ^(get_goal "Lannot")
+Proof
+  rw [evaluate_def]
+QED
+
+Theorem evaluate_ok_pmatch_Nil:
+  ^(get_goal "[]:(pat # exp) list")
+Proof
+  rw [evaluate_def] \\ gs []
+QED
+
+Theorem pmatch_ok:
+  pmatch env.c s.refs p v ws = Match env1 ∧
+  state_ok s ∧
+  env_ok s env ∧
+  v_ok s v ∧
+  EVERY (v_ok s) (MAP SND ws) ⇒
+    EVERY (v_ok s) (MAP SND env1)
+Proof
+  rw [state_ok_def, env_ok_def, v_ok_def, env_rel_def, state_rel_def]
+  \\ drule (CONJUNCT1 pmatch_update)
+  \\ rpt (disch_then drule) \\ gs []
+  \\ rpt (disch_then drule) \\ gs []
+  \\ disch_then (qspecl_then [‘s.refs’, ‘ws’] mp_tac) \\ simp []
+  \\ gs [EVERY_MAP, EVERY2_MAP, LIST_REL_EL_EQN, EVERY_EL, v_ok_def]
+  \\ rw [ELIM_UNCURRY]
+QED
+
+Theorem evaluate_ok_pmatch_Cons:
+  ^(get_goal "_::_:(pat # exp) list")
+Proof
+  rw [evaluate_def] \\ gs [CaseEqs ["match_result"]]
+  \\ rename1 ‘env_ok st (env with v := nsAppend (alist_to_ns env1) env.v)’
+  \\ drule pmatch_ok \\ rw [] \\ gs []
+  \\ ‘env_ok st (env with v := nsAppend (alist_to_ns env1) env.v)’
+    by (gs [env_ok_def, env_rel_def]
+        \\ irule nsAll2_nsAppend \\ gs []
+        \\ irule nsAll2_alist_to_ns
+        \\ gs [EVERY2_MAP, EVERY_EL]
+        \\ rw [LIST_REL_EL_EQN, ELIM_UNCURRY]
+        \\ gs [GSYM v_ok_def, EL_MAP])
+  \\ drule_all_then assume_tac evaluate_env_ok_mono \\ gs []
+  \\ gs [env_ok_def]
+  \\ drule_then assume_tac (CONJUNCT1 evaluate_next_type_stamp_mono)
+  \\ drule_then assume_tac (CONJUNCT1 evaluate_next_exn_stamp_mono)
+  \\ drule_then assume_tac (CONJUNCT1 evaluate_refs_length_mono)
+  \\ irule env_rel_update
+  \\ first_assum (irule_at Any)
+  \\ gs [FUN_FMAP_SUBMAP_SUBSET, COUNT_MONO]
+QED
+
+Theorem evaluate_ok_decs_Nil:
+  ^(get_goal "[]:dec list")
+Proof
+  rw [evaluate_decs_def, extend_dec_env_def]
+  \\ gs [env_ok_def, env_rel_def, ctor_rel_def]
+QED
+
+(*
+Theorem evaluate_ok_decs_Cons:
+  ^(get_goal "_::_::_:dec list")
+Proof
+  rw [evaluate_decs_def]
+  \\ gvs [CaseEqs ["prod", "result"], PULL_EXISTS]
+  \\ first_x_assum (drule_all_then strip_assume_tac) \\ gs []
+  \\ Cases_on ‘res1’ \\ gs []
+  >~ [‘res_rel _ _ (Rerr _) (Rerr _)’] >- (
+    first_assum (irule_at Any) \\ gs []
+    \\ first_assum (irule_at Any) \\ gs [])
+  \\ drule_all_then assume_tac env_rel_update
+  \\ dxrule_then (drule_then assume_tac) env_rel_extend_dec_env
+  \\ first_x_assum (drule_all_then strip_assume_tac)
+  \\ first_assum (irule_at (Pat ‘state_rel’))
+  \\ first_assum (irule_at Any)
+  \\ irule_at Any EQ_REFL
+  \\ irule_at Any SUBMAP_TRANS \\ first_assum (irule_at Any) \\ gs []
+  \\ irule_at Any SUBMAP_TRANS \\ first_assum (irule_at Any) \\ gs []
+  \\ irule_at Any SUBMAP_TRANS \\ first_assum (irule_at Any) \\ gs []
+  \\ gs [combine_dec_result_def]
+  \\ rpt CASE_TAC \\ gs []
+  \\ gs [extend_dec_env_def]
+  \\ gs [env_rel_def, ctor_rel_def]
+  \\ irule_at Any nsAll2_nsAppend
+  \\ irule_at Any nsAll2_nsAppend \\ gs []
+  \\ irule_at Any nsAll2_mono
+  \\ first_assum (irule_at Any) \\ gs []
+  \\ irule_at Any nsAll2_mono
+  \\ first_assum (irule_at Any) \\ gs []
+  \\ simp [FORALL_PROD]
+  \\ rw [] \\ (irule_at Any stamp_rel_update ORELSE irule_at Any v_rel_update)
+  \\ gs [SF SFY_ss]
+QED
+
+Theorem evaluate_ok_decs_Dlet:
+  ^(get_goal "Dlet")
+Proof
+  rw [evaluate_decs_def]
+  >~ [‘¬ALL_DISTINCT _’] >- (
+    first_assum (irule_at Any) \\ gs [SF SFY_ss])
+  \\ gvs [CaseEqs ["prod", "result"], PULL_EXISTS]
+  \\ first_x_assum (drule_all_then strip_assume_tac) \\ gs []
+  \\ Cases_on ‘res1’ \\ gs []
+  >~ [‘res_rel _ _ (Rerr err1) (Rerr err2)’] >- (
+    Cases_on ‘err1’ \\ Cases_on ‘err2’ \\ gs []
+    \\ first_assum (irule_at Any) \\ gs [SF SFY_ss])
+  \\ first_assum (irule_at Any) \\ gs [SF SFY_ss]
+  \\ drule_then strip_assume_tac evaluate_sing \\ gvs []
+  \\ ‘∃res. pmatch env.c s1.refs p x [] = res’ by gs []
+  \\ drule_all_then assume_tac env_rel_update
+  \\ gs [state_rel_def, env_rel_def]
+  \\ drule (CONJUNCT1 pmatch_update)
+  \\ rpt (disch_then drule) \\ simp []
+  \\ rpt (disch_then drule) \\ rw []
+  \\ rename1 ‘v_rel _ _ _ x y’
+  \\ Cases_on ‘pmatch env.c s1.refs p x []’
+  \\ Cases_on ‘pmatch env1.c t1.refs p y []’ \\ gs []
+  \\ rw [v_rel_def, bind_exn_v_def, Once stamp_rel_cases, bind_stamp_def,
+         ctor_rel_def]
+  \\ irule nsAll2_alist_to_ns \\ gs []
+QED
+
+Theorem evaluate_ok_decs_Dletrec:
+  ^(get_goal "Dletrec")
+Proof
+  rw [evaluate_decs_def]
+  >~ [‘¬ALL_DISTINCT _’] >- (
+    first_assum (irule_at Any) \\ gs [])
+  \\ gvs [CaseEqs ["prod", "result"], PULL_EXISTS]
+  \\ first_assum (irule_at Any) \\ gs []
+  \\ gs [env_rel_def, ctor_rel_def, PULL_EXISTS, SF SFY_ss,
+         semanticPrimitivesPropsTheory.build_rec_env_merge]
+  \\ irule_at Any nsAll2_alist_to_ns
+  \\ gs [EVERY2_MAP, LAMBDA_PROD]
+  \\ rw [v_rel_def, LIST_REL_EL_EQN, ELIM_UNCURRY, env_rel_def, ctor_rel_def]
+QED
+
+Theorem state_rel_with_next_type_stamp:
+  state_rel l fr ft fe s t ⇒
+    state_rel l fr
+      (ft ⊌ FUN_FMAP (λn. n - s.next_type_stamp + t.next_type_stamp)
+                     (IMAGE ($+ s.next_type_stamp) (count extra))) fe
+      (s with next_type_stamp := extra + s.next_type_stamp)
+      (t with next_type_stamp := extra + t.next_type_stamp)
+Proof
+  simp [state_rel_def] \\ strip_tac
+  \\ gs [flookup_thm, FUNION_DEF]
+  \\ conj_tac
+  >- (
+    qpat_x_assum ‘INJ ($' ft) _ _’ mp_tac
+    \\ qpat_x_assum ‘FDOM ft = _’ mp_tac
+    \\ rpt (pop_assum kall_tac)
+    \\ rw [INJ_IFF, FUNION_DEF]
+    \\ rw [FUN_FMAP_DEF] \\ gs [CaseEq "bool"]
+    \\ res_tac \\ fs [])
+  \\ once_rewrite_tac [ADD_COMM] \\ simp [count_add]
+  \\ qx_gen_tac ‘m’ \\ strip_tac
+  \\ last_x_assum drule \\ rw []
+  \\ irule ref_rel_mono
+  \\ first_assum (irule_at Any) \\ rw []
+  \\ irule v_rel_update
+  \\ first_assum (irule_at (Pat ‘v_rel’))
+  \\ gs [SUBMAP_FUNION_ID]
+QED
+
+Theorem state_rel_with_next_exn_stamp:
+  state_rel l fr ft fe s t ⇒
+    state_rel l fr ft
+      (fe ⊌ FUN_FMAP (λn. n - s.next_exn_stamp + t.next_exn_stamp)
+                     (IMAGE ($+ s.next_exn_stamp) (count extra)))
+      (s with next_exn_stamp := extra + s.next_exn_stamp)
+      (t with next_exn_stamp := extra + t.next_exn_stamp)
+Proof
+  simp [state_rel_def] \\ strip_tac
+  \\ gs [flookup_thm, FUNION_DEF]
+  \\ conj_tac
+  >- (
+    qpat_x_assum ‘INJ ($' fe) _ _’ mp_tac
+    \\ qpat_x_assum ‘FDOM fe = _’ mp_tac
+    \\ rpt (pop_assum kall_tac)
+    \\ rw [INJ_IFF, FUNION_DEF]
+    \\ rw [FUN_FMAP_DEF] \\ gs [CaseEq "bool"]
+    \\ res_tac \\ fs [])
+  \\ once_rewrite_tac [ADD_COMM] \\ simp [count_add]
+  \\ qx_gen_tac ‘m’ \\ strip_tac
+  \\ last_x_assum drule \\ rw []
+  \\ irule ref_rel_mono
+  \\ first_assum (irule_at Any) \\ rw []
+  \\ irule v_rel_update
+  \\ first_assum (irule_at (Pat ‘v_rel’))
+  \\ gs [SUBMAP_FUNION_ID]
+QED
+
+Theorem evaluate_ok_decs_Dtype:
+  ^(get_goal "Dtype")
+Proof
+  rw [evaluate_decs_def]
+  >~ [‘¬EVERY check_dup_ctors _’] >- (
+    first_assum (irule_at (Pat ‘state_rel’))
+    \\ gs [])
+  \\ drule_all_then (qspec_then ‘LENGTH tds’ assume_tac)
+                    state_rel_with_next_type_stamp
+  \\ rw []
+  \\ first_assum (irule_at Any)
+  \\ gs [SUBMAP_FUNION_ID]
+  \\ gvs [env_rel_def, ctor_rel_def, state_rel_def]
+  \\ qpat_x_assum ‘INJ ($' (FUNION _ _)) _ _’ mp_tac
+  \\ qpat_x_assum ‘INJ ($' ft) _ _’ mp_tac
+  \\ qpat_x_assum ‘FDOM ft = _’ mp_tac
+  \\ rpt (pop_assum kall_tac)
+  \\ rename1 ‘_ _ (build_tdefs n _) (_ m _)’
+  \\ qid_spec_tac ‘ft’
+  \\ qid_spec_tac ‘m’
+  \\ qid_spec_tac ‘tds’
+  \\ qid_spec_tac ‘n’
+  \\ ho_match_mp_tac build_tdefs_ind
+  \\ rw [build_tdefs_def]
+  \\ irule nsAll2_nsAppend \\ gs []
+  \\ irule_at Any nsAll2_alist_to_ns \\ gs []
+  \\ conj_tac
+  >- (
+    gs [build_constrs_def, EVERY2_MAP, LAMBDA_PROD, stamp_rel_cases]
+    \\ gvs [LIST_REL_EL_EQN] \\ rw []
+    \\ rpt (pairarg_tac \\ gvs [])
+    \\ gs [flookup_thm]
+    \\ conj_tac >- (qexists_tac ‘0’ \\ simp [])
+    \\ simp [FUNION_DEF]
+    \\ qmatch_goalsub_abbrev_tac ‘FUN_FMAP f D’
+    \\ ‘n ∈ D’
+      by (gs [Abbr ‘D’] \\ qexists_tac ‘0’ \\ gs [])
+    \\ ‘FINITE D’
+      by gs [Abbr ‘D’]
+    \\ drule_then (qspec_then ‘f’ mp_tac) FUN_FMAP_DEF \\ rw []
+    \\ gs [Abbr ‘f’])
+  \\ gs [ADD1]
+  \\ ‘FDOM (ft |+ (n, m)) = count (n + 1)’
+    by rw [EXTENSION]
+  \\ ‘INJ ($' (ft |+ (n, m))) (count (n + 1)) (count (m + 1))’
+    by (gs [INJ_IFF, FAPPLY_FUPDATE_THM]
+        \\ rw [] \\ gs []
+        \\ rename1 ‘x < n + 1’ \\ ‘x < n’ by gs []
+        \\ res_tac \\ fs [])
+  \\ ‘INJ ($' (FUNION (ft |+ (n,m)) (FUN_FMAP (λx. x - (n + 1) + (m + 1))
+                                    (IMAGE ($+ (n + 1)) (count (LENGTH tds))))))
+                                    (count (n + (LENGTH tds + 1)))
+                                    (count (m + (LENGTH tds + 1)))’
+    by (qmatch_goalsub_abbrev_tac ‘($' ft')’
+        \\ ‘∀k. k < n + LENGTH tds + 1 ⇒
+                if k < n then ft' ' k = ft ' k else
+                if k = n then ft' ' k = m else
+                ft' ' k = k + m - n’
+          by (csimp [Abbr ‘ft'’, FUNION_DEF, FAPPLY_FUPDATE_THM]
+              \\ rw [DISJ_EQ_IMP]
+              \\ qmatch_goalsub_abbrev_tac ‘FUN_FMAP f D’
+              \\ ‘k ∈ D’
+                by (gs [Abbr ‘D’] \\ qexists_tac ‘k - n - 1’ \\ gs [])
+              \\ ‘FINITE D’
+                by gs [Abbr ‘D’]
+              \\ drule_then (qspec_then ‘f’ mp_tac) FUN_FMAP_DEF \\ rw []
+              \\ gs [Abbr ‘f’])
+        \\ qpat_x_assum ‘INJ ($' ft) _ _’ mp_tac
+        \\ rw [INJ_IFF]
+        >- (
+          gs [] \\ res_tac \\ fs [COND_EXPAND]
+          \\ res_tac \\ fs [])
+        \\ rw [EQ_IMP_THM] \\ gs []
+        \\ first_assum drule_all
+        \\ ntac 2 (pop_assum mp_tac)
+        \\ first_x_assum drule_all
+        \\ rw [] \\ gs []
+        \\ res_tac \\ fs [])
+  \\ first_x_assum (drule_then (qspec_then ‘m + 1’ mp_tac))
+  \\ rw []
+  \\ irule nsAll2_mono
+  \\ first_assum (irule_at Any) \\ gs []
+  \\ simp [FORALL_PROD]
+  \\ rw [stamp_rel_cases]
+  \\ gs [flookup_thm, FUN_FMAP_DEF, FUNION_DEF, FAPPLY_FUPDATE_THM, SF CONJ_ss]
+  \\ Cases_on ‘m1 = n’ \\ gvs []
+  \\ conj_tac >- (qexists_tac ‘0’ \\ simp [])
+  \\ qmatch_goalsub_abbrev_tac ‘FUN_FMAP f D’
+  \\ ‘m1 ∈ D’
+    by (gs [Abbr ‘D’] \\ qexists_tac ‘0’ \\ gs [])
+  \\ ‘FINITE D’
+    by gs [Abbr ‘D’]
+  \\ drule_then (qspec_then ‘f’ mp_tac) FUN_FMAP_DEF \\ rw []
+  \\ gs [Abbr ‘f’]
+QED
+
+Theorem evaluate_ok_decs_Dtabbrev:
+  ^(get_goal "Dtabbrev")
+Proof
+  rw [evaluate_decs_def]
+  \\ first_assum (irule_at Any) \\ gs []
+  \\ simp [env_rel_def, ctor_rel_def]
+QED
+
+Theorem state_rel_declare_env[local]:
+  state_rel l fr ft fe s t ⇒
+    (∀env. declare_env s.eval_state env = NONE) ∧
+    (∀env. declare_env t.eval_state env = NONE)
+Proof
+  rw [state_rel_def, declare_env_def]
+QED
+
+Theorem evaluate_ok_decs_Denv:
+  ^(get_goal "Denv")
+Proof
+  rw [evaluate_decs_def]
+  \\ drule_then assume_tac state_rel_declare_env \\ gs []
+  \\ first_assum (irule_at Any) \\ gs []
+QED
+
+Theorem evaluate_ok_decs_Dexn:
+  ^(get_goal "Dexn")
+Proof
+  rw [evaluate_decs_def]
+  \\ gvs [CaseEqs ["option", "prod"]]
+  \\ drule_then (qspec_then ‘1’ assume_tac)
+                state_rel_with_next_exn_stamp \\ gs []
+  \\ first_assum (irule_at (Pat ‘state_rel’)) \\ gs []
+  \\ simp [SUBMAP_FUNION_ID]
+  \\ gs [env_rel_def, ctor_rel_def, stamp_rel_cases, flookup_thm,
+         FUNION_DEF, state_rel_def, FUN_FMAP_DEF]
+QED
+
+Theorem evaluate_ok_decs_Dmod:
+  ^(get_goal "Dmod")
+Proof
+  rw [evaluate_decs_def]
+  \\ gvs [CaseEqs ["option", "prod", "result"]]
+  \\ first_x_assum (drule_all_then strip_assume_tac)
+  \\ Cases_on ‘res1’ \\ gs []
+  \\ first_assum (irule_at Any) \\ gs []
+  \\ gs [env_rel_def, ctor_rel_def]
+QED
+
+Theorem evaluate_ok_decs_Dlocal:
+  ^(get_goal "Dlocal")
+Proof
+  rw [evaluate_decs_def]
+  \\ gvs [CaseEqs ["option", "prod", "result"]]
+  \\ first_x_assum (drule_all_then strip_assume_tac)
+  \\ drule_all_then assume_tac env_rel_update
+  \\ Cases_on ‘res1’ \\ gs []
+  >~ [‘res_rel _ _ (Rerr _) (Rerr _)’] >- (
+    first_assum (irule_at Any)
+    \\ gs [])
+  \\ dxrule_then (drule_then assume_tac) env_rel_extend_dec_env
+  \\ first_x_assum (drule_all_then strip_assume_tac)
+  \\ first_assum (irule_at Any) \\ gs []
+  \\ irule_at Any SUBMAP_TRANS \\ first_assum (irule_at Any) \\ gs []
+  \\ irule_at Any SUBMAP_TRANS \\ first_assum (irule_at Any) \\ gs []
+  \\ irule_at Any SUBMAP_TRANS \\ first_assum (irule_at Any) \\ gs []
+QED
+
+Theorem evaluate_ok:
+  ^(evaluate_ok ())
+Proof
+  match_mp_tac (the_ind_thm ())
+  \\ rpt conj_tac \\ rpt gen_tac
+  \\ rewrite_tac [evaluate_ok_Nil, evaluate_ok_Cons,
+                  evaluate_ok_Lit, evaluate_ok_Raise,
+                  evaluate_ok_Handle, evaluate_ok_Con,
+                  evaluate_ok_Var, evaluate_ok_Fun,
+                  evaluate_ok_App, evaluate_ok_Log,
+                  evaluate_ok_If, evaluate_ok_Mat,
+                  evaluate_ok_Let, evaluate_ok_Letrec,
+                  evaluate_ok_Tannot, evaluate_ok_Lannot,
+                  evaluate_ok_pmatch_Nil, evaluate_ok_pmatch_Cons,
+                  evaluate_ok_decs_Nil, evaluate_ok_decs_Cons,
+                  evaluate_ok_decs_Dlet, evaluate_ok_decs_Dletrec,
+                  evaluate_ok_decs_Dtype,
+                  evaluate_ok_decs_Dtabbrev,
+                  evaluate_ok_decs_Denv, evaluate_ok_decs_Dexn,
+                  evaluate_ok_decs_Dmod, evaluate_ok_decs_Dlocal]
+QED
+
+ *)
+
+
+
+
+
+
+
+
+
+
+
+
+
+
+(* -------------------------------------------------------------------------
+ *
+ * ------------------------------------------------------------------------- *)
 
 Theorem state_rel_init:
   state_rel 0 FEMPTY (FUN_FMAP I (count 2)) (FUN_FMAP I (count 4))
@@ -99,3 +1801,4 @@ Proof
 QED
 
 val _ = export_theory();
+
